theories/Utils.v
@@ -144,11 +144,11 @@ Notation "x '+++' y" := (appne x y) (at level 60, right associativity).
 (** finite multisets are represented with ordered lists with multiplicities *)
 Definition mset A := nelist (A*positive).
 
-Definition copy_mset {X} n (l: mset X): mset X :=
-  match n with
-  | xH => l
-  | _ => nelist_map (fun vm => let '(v,m):=vm in (v,Pmult n m)) l
-  end.
+    Definition copy_mset {X} n (l: mset X): mset X :=
+      match n with
+        | xH => l
+        | _ => nelist_map (fun vm => let '(v,m):=vm in (v,Pmult n m)) l
+      end.
 
 (** lexicographic composition of comparisons (this is a notation to keep it lazy) *)
 Notation lex e f := (match e with Eq => f | _ => e end).  
@@ -320,3 +320,17 @@ Section copy.
   Qed.
 
 End copy.
+
+(** * Translate Heterogenous to Homogenous *)
+
+Section H.
+
+  Variable Obj : Type.
+  Variable Arr : Obj -> Obj -> Type.
+  Variable R : forall A B, Arr A B -> Arr A B -> Prop.
+  Variable f : forall A B C, Arr B C -> Arr A B -> Arr A C.
+  
+  Lemma HAssociative_Associative A: HAssociative R f -> Associative (@R A A) (@f A A A).
+  Proof. cbv. intuition. Qed.
+  
+End H.
